coq/proof/SimulationValid.v
@@ -224,7 +224,7 @@ Proof.
       * econs 1. econs; eauto. rewrite lookupBlockViaLabelFromFdef_spec. ss.
       * right. apply CIH. econs; ss; eauto; ss; eauto.
     + (* switch *)
-      destruct (list_const_l_dec l0 l1); ss. subst. (* TODO *)
+      destruct (list_const_l_dec l0 l1); ss. subst.
       exploit nerror_nfinal_nstuck; eauto. i. des. inv x0.
       exploit InvState.Rel.inject_value_spec; eauto.
       { rewrite InvState.Unary.sem_valueT_physical. eauto. }
@@ -233,28 +233,29 @@ Proof.
       eapply _sim_local_step.
       { admit. (* tgt not stuck *) }
       i. inv STEP. unfold valid_phinodes in *. simtac.
-      (* rewrite add_terminator_cond_switch in *. *)
-      (* rewrite lookupBlockViaLabelFromFdef_spec in *. *)
-      admit.
+      exploit add_terminator_cond_switch; eauto. i. des.
+      rewrite lookupBlockViaLabelFromFdef_spec in *.
+      admit. (* similar to conditional branch *)
     + (* unreachable *)
       exploit nerror_nfinal_nstuck; eauto. i. des. inv x0.
   - (* cmd *)
     destruct (Instruction.isCallInst c) eqn:CALL.
     + (* call *)
-      admit.
-      (* exploit postcond_cmd_is_call; eauto. i. *)
-      (* destruct c; ss. destruct c0; ss. *)
-      (* hexploit postcond_call_sound; try exact COND; eauto; *)
-      (*   (try instantiate (2 := (mkState (mkEC _ _ _ _ _ _) _ _))); ss; eauto; ss. *)
-      (* i. des. subst. do 24 simtac0. des. *)
-      (* eapply _sim_local_call; ss; eauto; ss. *)
-      (* i. exploit RETURN; eauto. *)
-      (* exploit apply_infrules_sound; eauto; ss. i. des. *)
-      (* exploit reduce_maydiff_sound; eauto; ss. i. des. *)
-      (* exploit implies_sound; eauto; ss. i. des. *)
-      (* exists locals2_tgt, 0%nat, invmem1. splits; ss. *)
-      (* * etransitivity; eauto. *)
-      (* * right. apply CIH. econs; eauto. *)
+      exploit postcond_cmd_is_call; eauto. i.
+      destruct c; ss. destruct c0; ss.
+      hexploit postcond_call_sound; try exact COND; eauto;
+        (try instantiate (2 := (mkState (mkEC _ _ _ _ _ _) _ _))); ss; eauto; ss.
+      i. des. subst. do 24 simtac0. des.
+      eapply _sim_local_call; ss; eauto; ss.
+      i. exploit RETURN; eauto.
+      { admit. (* connect memory_blocks_of and uniqs *) }
+      i. des.
+      exploit apply_infrules_sound; eauto; ss. i. des.
+      exploit reduce_maydiff_sound; eauto; ss. i. des.
+      exploit implies_sound; eauto; ss. i. des.
+      exists locals2_tgt, 0%nat, invmem1. splits; ss.
+      * etransitivity; eauto.
+      * right. apply CIH. econs; eauto.
     + (* non-call *)
       eapply _sim_local_step.
       { admit. (* tgt not stuck *) }
@@ -348,7 +349,6 @@ Proof.
     destruct (initFunTable mem0 id0); eauto.
 Qed.
 
-(* TODO: extract lemma for module initialization *)
 Lemma valid_sim_module m_hint:
   (fun p q => valid_module m_hint p q = Some true) <2= sim_module.
 Proof.
